src/ShouldBuild.v
@@ -5,4 +5,5 @@ From RecoveryRefinement Require Import Database.Simple.SimpleDb.
 From RecoveryRefinement Require Import CSL.RefinementAdequacy.
 From RecoveryRefinement Require Import CSL.Lifting.
 From RecoveryRefinement Require Import Examples.ExMach.WeakestPre.
+From RecoveryRefinement Require Import Examples.ExMach.RefinementAdequacy.
 From RecoveryRefinement Require Import Examples.StatDb.Refinement.
